<?xml version="1.0"?>

<!DOCTYPE RDF [
   <!ENTITY rdf  "http://www.w3.org/1999/02/22-rdf-syntax-ns">
   <!ENTITY rdfs "http://www.w3.org/2000/01/rdf-schema">
   <!ENTITY xsd  "http://www.w3.org/2001/XMLSchema">
   <!ENTITY rdfg "http://www.w3.org/2004/03/trix/rdfg-1">
   <!ENTITY xmlsig "http://www.w3.org/2000/09/xmldsig">
   <!ENTITY swp  "http://www.w3.org/2004/03/trix/swp-2">
]>

<!--
   
########################################################
         Semantic Web Publishing Vocabulary
########################################################   
   
Version: 0.2.1
Date: Nov 30, 2004

Authors: 
   Jeremy J. Carroll, 
   Christian Bizer, 
   Patrick Hayes,
   Patrick Stickler
   
Contents:
   1. SWP Base Vocabulary
   2. SWP Signature-Related Vocabulary
   3. SWP Signature-Related Algorithms

        
Changes:
   Nov 30, 2004: Added signature related vocabulary and algorithms.
   May 20, 2004: Initial version of the vocabulary.
         
-->

<rdf:RDF
  xml:base="&swp;/"
   xmlns:rdf="&rdf;#"
   xmlns:rdfs="&rdfs;#"
   xmlns:xsd="&xsd;#"
   xmlns:rdfg="&rdfg;/"
   xmlns:swp="&swp;/">


<!-- 
########################################################  
           1. SWP Base Vocabulary 
########################################################  
-->

   <rdfs:Class rdf:about="&swp;/Authority">
      <rdfs:label>Authority</rdfs:label>
      <rdfs:comment>
An authority, or origin, of a graph; such as a person or company.
      </rdfs:comment>
   </rdfs:Class>

   <rdfs:Class rdf:about="&swp;/Warrant">
      <rdfs:label>Warrant</rdfs:label>
      <rdfs:comment>
A relationship between an authority and a graph, in which the authority is in
some way an origin of that graph. Warrants may include a digital signature of
the graph by the authority.
      </rdfs:comment>
   </rdfs:Class>

   <rdf:Property rdf:about="&swp;/assertedBy">
      <rdfs:label>asserted by</rdfs:label>
      <rdfs:comment>
The subject graph originates from and is asserted by the authority specified
for the object warrant. The statements expressed in the graph are taken to be
claims made by that authority. This property has performative semantics.
      </rdfs:comment>
      <rdfs:domain rdf:resource="&rdfg;/Graph"/>
      <rdfs:range rdf:resource="&swp;/Warrant"/>
   </rdf:Property>

   <rdf:Property rdf:about="&swp;/quotedBy">
      <rdfs:label>quoted by</rdfs:label>
      <rdfs:comment>
The subject graph originates from the authority specified for the object warrant.
The statements expressed in the graph are not taken to be claims made by that
authority, insofar as any statement using this property is concerned.
      </rdfs:comment>
      <rdfs:domain rdf:resource="&rdfg;/Graph"/>
      <rdfs:range rdf:resource="&swp;/Warrant"/>
   </rdf:Property>

   <rdf:Property rdf:about="&swp;/authority">
      <rdfs:label>authority</rdfs:label>
      <rdfs:comment>
The object authority is the origin of the graph with which the subject warrant
is associated.
      </rdfs:comment>
      <rdfs:domain rdf:resource="&swp;/Warrant"/>
      <rdfs:range rdf:resource="&swp;/Authority"/>
   </rdf:Property>
   
   <rdf:Property rdf:about="&swp;/validUntil">
      <rdfs:label>valid from</rdfs:label>
      <rdfs:comment>
Defines a point in time until which the warrant is valid.
      </rdfs:comment>
      <rdfs:domain rdf:resource="&swp;/Warrant"/>
      <rdfs:range rdf:resource="&xsd;#dateTime"/>
   </rdf:Property>

   <rdf:Property rdf:about="&swp;/validFrom">
      <rdfs:label>valid from</rdfs:label>
      <rdfs:comment>
Defines a point in time after which the warrant is valid.
      </rdfs:comment>
      <rdfs:domain rdf:resource="&swp;/Warrant"/>
      <rdfs:range rdf:resource="&xsd;#dateTime"/>
   </rdf:Property>

<!-- 
########################################################  
       2. SWP Signature Related Vocabulary 
########################################################  
-->

<!-- Signing Warrants -->

   <rdf:Property rdf:about="&swp;/signature">
      <rdfs:label>signature</rdfs:label>
      <rdfs:comment>
The object is the signature to be used to authenticate the graph with which the
subject warrant is associated.
      </rdfs:comment>
      <rdfs:domain rdf:resource="&swp;/Warrant"/>
      <rdfs:range rdf:resource="&xsd;#base64Binary"/>
   </rdf:Property>

   <rdf:Property rdf:about="&swp;/signatureMethod">
      <rdfs:label>signature method</rdfs:label>
      <rdfs:comment>
The object is the signature method by which the signature specified for the
warrant subject was constructed.
      </rdfs:comment>
      <rdfs:domain rdf:resource="&swp;/Warrant"/>
      <rdfs:range rdf:resource="&swp;/SignatureMethod"/>
   </rdf:Property>


<!-- Defining Signature Methods -->

   <rdfs:Class rdf:about="&swp;/SignatureMethod">
      <rdfs:label>Signature Method</rdfs:label>
      <rdfs:comment>
A method used for creating a signature used to authenticate a graph.
Signature methods define an canonicalization method and a signature algorithm.
      </rdfs:comment>
   </rdfs:Class>

   <rdfs:Class rdf:about="&swp;/CanonicalizationAlgorithm">
      <rdfs:label>Canonicalization Algorithm</rdfs:label>
      <rdfs:comment>
An algorithm used to transform a graph to a canonical form.
      </rdfs:comment>
   </rdfs:Class>

   <rdfs:Class rdf:about="&swp;/SignatureAlgorithm">
      <rdfs:label>Signature Algorithm</rdfs:label>
      <rdfs:comment>
An algorithm to compute a hash digest from some data and to sign the digest.
      </rdfs:comment>
   </rdfs:Class>

   <rdf:Property rdf:about="&swp;/canonicalizationAlgorithm">
      <rdfs:label>canonicalization algorithm</rdfs:label>
      <rdfs:comment>
Canonicalization method used by this signature or digest method.
      </rdfs:comment>
      <rdfs:range rdf:resource="&swp;/CanonicalizationAlgorithm"/>
   </rdf:Property>

   <rdf:Property rdf:about="&swp;/signatureAlgorithm">
      <rdfs:label>signature algorithm</rdfs:label>
      <rdfs:comment>
Signature algorithm used by this signature method.
      </rdfs:comment>
      <rdfs:domain rdf:resource="&swp;/SignatureMethod"/>
      <rdfs:range rdf:resource="&swp;/SignatureAlgorithm"/>
   </rdf:Property>


<!-- Graph Digests -->

   <rdf:Property rdf:about="&swp;/digest">
      <rdfs:label>digest</rdfs:label>
      <rdfs:comment>
The object contains a digest value for the subject graph.
      </rdfs:comment>
      <rdfs:domain rdf:resource="&rdfg;/Graph"/>
      <rdfs:range rdf:resource="&xsd;#base64Binary"/>
   </rdf:Property>

   <rdf:Property rdf:about="&swp;/digestMethod">
      <rdfs:label>digest method</rdfs:label>
      <rdfs:comment>
The object is the digest method by which the digest value specified for the
graph subject was constructed.
      </rdfs:comment>
      <rdfs:domain rdf:resource="&rdfg;/Graph"/>
      <rdfs:range rdf:resource="&swp;/DigestMethod"/>
   </rdf:Property>


<!-- Defining Digest Methods -->

   <rdfs:Class rdf:about="&swp;/DigestMethod">
      <rdfs:label>Digest Method</rdfs:label>
      <rdfs:comment>
A method used for computing a digest a graph.
Digest method defines a canonicalization alorithm and a digest algorithm.
      </rdfs:comment>
   </rdfs:Class>

   <rdfs:Class rdf:about="&swp;/DigestAlgorithm">
      <rdfs:label>Digest Algorithm</rdfs:label>
      <rdfs:comment>
A hash algorithm to compute a digest from some data.
      </rdfs:comment>
   </rdfs:Class>

   <rdf:Property rdf:about="&swp;/digestAlgorithm">
      <rdfs:label>signature algorithm</rdfs:label>
      <rdfs:comment>
Digest algorithm used by this digest method.
      </rdfs:comment>
      <rdfs:domain rdf:resource="&swp;/DigestMethod"/>
      <rdfs:range rdf:resource="&swp;/DigestAlgorithm"/>
   </rdf:Property>


<!-- Publishing Key and Certification Information -->

   <rdf:Property rdf:about="&swp;/hasKey">
      <rdfs:label>has key</rdfs:label>
      <rdfs:comment>
The object is some kind of public key which belongs to the authority.
      </rdfs:comment>
      <rdfs:domain rdf:resource="&swp;/Authority"/>
      <rdfs:range rdf:resource="&swp;/Key"/>
   </rdf:Property>

   <rdf:Property rdf:about="&swp;/keyInfo">
      <rdfs:label>key info</rdfs:label>
      <rdfs:comment>
The object is some kind of public key which can be used to validate the signature attached to the warrant.
      </rdfs:comment>
      <rdfs:domain rdf:resource="&swp;/Warrant"/>
      <rdfs:range rdf:resource="&swp;/Key"/>
   </rdf:Property>

   <rdf:Property rdf:about="&swp;/certificate">
      <rdfs:label>certificate</rdfs:label>
      <rdfs:comment>
The object is a binary (ASN.1 DER) X.509 certificate containing the public key of the authority.
This property is similar to the xmldsig#rawX509Certificate property. 
An alternative to the use of this property is to use swp:hasKey together with swp:X509Certificate.
      </rdfs:comment>
      <rdfs:domain rdf:resource="&swp;/Authority"/>
      <rdfs:range rdf:resource="&xsd;#base64Binary"/>
   </rdf:Property>

<!-- Representing Keys and Certificates -->

   <rdfs:Class rdf:about="&swp;/Key">
      <rdfs:label>Key</rdfs:label>
      <rdfs:comment>
Superclass of all classes representing cryptographic key information.
      </rdfs:comment>
   </rdfs:Class>

   <rdfs:Class rdf:about="&swp;/DSAKey">
      <rdfs:label>DSA key</rdfs:label>
      <rdfs:subClassOf rdf:resource="&swp;/Key"/>
      <rdfs:comment>
A DSA key as defined by XML-Signature in http://www.w3.org/TR/xmldsig-core/
The XML-Signature P Q G Y J Seed and PgenCounter properties should be used to describe the key.
      </rdfs:comment>
   </rdfs:Class>

   <rdfs:Class rdf:about="&swp;/RSAKey">
      <rdfs:label>RSA key</rdfs:label>
      <rdfs:subClassOf rdf:resource="&swp;/Key"/>
      <rdfs:comment>
A RSA key as defined by XML-Signature in http://www.w3.org/TR/xmldsig-core/
The XML-Signature Modulus and Exponent properties should be used to describe the key.
      </rdfs:comment>
   </rdfs:Class>

   <rdfs:Class rdf:about="&swp;/PGPKey">
      <rdfs:label>PGP key</rdfs:label>
      <rdfs:subClassOf rdf:resource="&swp;/Key"/>
      <rdfs:comment>
A PGP key as defined by XML-Signature in http://www.w3.org/TR/xmldsig-core/
The XML-Signature PGPKeyID and PGPKeyPacket properties should be used to describe the key.
      </rdfs:comment>
   </rdfs:Class>

   <rdfs:Class rdf:about="&swp;/X509Certificate">
      <rdfs:label>X509 Certificate</rdfs:label>
      <rdfs:subClassOf rdf:resource="&swp;/Key"/>
      <rdfs:comment>
A X509 certificate as defined by XML-Signature in http://www.w3.org/TR/xmldsig-core/
The XML-Signature X509IssuerSerial X509SubjectName X509SKI X509Certificate properties 
should be used to describe the certificate.
      </rdfs:comment>
   </rdfs:Class>

   <rdf:Property rdf:about="&swp;/certificationAuthority">
      <rdfs:label>certification authority</rdfs:label>
      <rdfs:comment>
The object is the certification authority which issed the X509 certificate.
      </rdfs:comment>
      <rdfs:domain rdf:resource="&swp;/X509Certificate"/>
      <rdfs:range rdf:resource="&swp;/CertificationAuthority"/>
   </rdf:Property>

   <rdfs:Class rdf:about="&swp;/CertificationAuthority">
      <rdfs:label>Certification Authority</rdfs:label>
      <rdfs:comment>
An authority which issues certificates.
      </rdfs:comment>
   </rdfs:Class>


<!-- 
########################################################  
        3. SWP Signature Related Algorithms 
########################################################  
-->

   <swp:CanonicalizationAlgorithm rdf:about="&swp;/JjcRdfC14N">
      <rdfs:label>Jeremy Carroll's RDF C14N Method</rdfs:label>
      <rdfs:comment>Jeremy Carroll's RDF C14N method described in 'Signing RDF Graphs' 
      http://www.hpl.hp.com/techreports/2003/HPL-2003-142.html</rdfs:comment>
   </swp:CanonicalizationAlgorithm>

   <swp:CanonicalizationAlgorithm rdf:about="&swp;/SaKaRdfC14N">
      <rdfs:label>Craig Sayers and Alan H. Karp's RDF C14N Method</rdfs:label>
      <rdfs:comment>Craig Sayers and Alan H. Karp's RDF C14N method described in 
       'Computing the digest of an RDF graph' http://www.hpl.hp.com/techreports/2003/HPL-2003-235.pdf</rdfs:comment>
   </swp:CanonicalizationAlgorithm>

   <swp:DigestAlgorithm rdf:about="&xmlsig;#sha1">
      <rdfs:label>SHA1</rdfs:label>
      <rdfs:comment>SHA1 as defined by XML-Signature in http://www.w3.org/TR/xmldsig-core/</rdfs:comment>
   </swp:DigestAlgorithm>

   <swp:SignatureAlgorithm rdf:about="&xmlsig;#dsa-sha1">
      <rdfs:label>DSA with SHA1(DSS)</rdfs:label>
      <rdfs:comment>DSA with SHA1 as defined by XML-Signature in http://www.w3.org/TR/xmldsig-core/</rdfs:comment>
   </swp:SignatureAlgorithm>

   <swp:SignatureAlgorithm rdf:about="&xmlsig;#rsa-sha1">
      <rdfs:label>RSA with SHA1</rdfs:label>
      <rdfs:comment>RSA with SHA1 as defined by XML-Signature in http://www.w3.org/TR/xmldsig-core/</rdfs:comment>
   </swp:SignatureAlgorithm>

   <swp:SignatureMethod rdf:about="&swp;/JjcRdfC14N-dsa-sha1">
      <rdfs:label>JjcRdfC14N-dsa-sha1</rdfs:label>
      <rdfs:comment>Jeremy's C14N method together with SHA1 and DSA</rdfs:comment>
      <swp:canonicalizationAlgorithm rdf:resource="&swp;/JjcRdfC14N"/>
      <swp:signatureAlgorithm rdf:resource="&xmlsig;#dsa-sha1"/>
   </swp:SignatureMethod>

   <swp:SignatureMethod rdf:about="&swp;/JjcRdfC14N-rsa-sha1">
      <rdfs:label>JjcRdfC14N-rsa-sha1</rdfs:label>
      <rdfs:comment>Jeremy's C14N method together with SHA1 and RSA</rdfs:comment>
      <swp:canonicalizationAlgorithm rdf:resource="&swp;/JjcRdfC14N"/>
      <swp:signatureAlgorithm rdf:resource="&xmlsig;#rsa-sha1"/>
   </swp:SignatureMethod>

   <swp:DigestMethod rdf:about="&swp;/JjcRdfC14N-sha1">
      <rdfs:label>JjcRdfC14N-sha1</rdfs:label>
      <rdfs:comment>Jeremy's C14N method together with SHA1</rdfs:comment>
      <swp:canonicalizationAlgorithm rdf:resource="&swp;/JjcRdfC14N"/>
      <swp:digestAlgorithm rdf:resource="&xmlsig;#sha1"/>
   </swp:DigestMethod>

</rdf:RDF>

